```
$$
\frac{1}{(1 + \sqrt{2^3})^{4}} + \sum_{n=1}^{\infty} \frac{(-1)^n \cdot n!}{2^n} + \int_{0}^{\pi} e^{i \theta} d\theta
$$
```
$$
\frac{1}{(1 + \sqrt{2^3})^{4}} + \sum_{n=1}^{\infty} \frac{(-1)^n \cdot n!}{2^n} + \int_{0}^{\pi} e^{i \theta} d\theta
$$




---




```
$
\frac{1}{(1 + \sqrt{2^3})^{4}} + \sum_{n=1}^{\infty} \frac{(-1)^n \cdot n!}{2^n} + \int_{0}^{\pi} e^{i \theta} d\theta
$
```
$
\frac{1}{(1 + \sqrt{2^3})^{4}} + \sum_{n=1}^{\infty} \frac{(-1)^n \cdot n!}{2^n} + \int_{0}^{\pi} e^{i \theta} d\theta
$




---




```
$
\frac{1}{(1 + \sqrt{2^3})^{4}} + \sum_{n=1}^{\infty} \frac{(-1)^n \cdot n!}{2^n} + \int_{0}^{\pi} e^{i \theta} d\theta

```
$
\frac{1}{(1 + \sqrt{2^3})^{4}} + \sum_{n=1}^{\infty} \frac{(-1)^n \cdot n!}{2^n} + \int_{0}^{\pi} e^{i \theta} d\theta
